Strengthen an invariant

semantics/alt_semantics/proofs/bigSmallInvariantsScript.sml
@@ -13,116 +13,125 @@ val _ = new_theory "bigSmallInvariants"
 (* ------ Auxiliary relations for proving big/small step equivalence ------ *)
 
 Inductive evaluate_ctxt:
-  evaluate_ctxt env s (Craise ()) v (s, Rerr (Rraise v)) ∧
+  evaluate_ctxt ck env s (Craise ()) v (s, Rerr (Rraise v)) ∧
 
-  evaluate_ctxt env s (Chandle () pes) v (s, Rval v) ∧
+  evaluate_ctxt ck env s (Chandle () pes) v (s, Rval v) ∧
 
-  (evaluate_list F env s1 es (s2, Rval vs2) ∧
+  (evaluate_list ck env s1 es (s2, Rval vs2) ∧
    do_opapp (REVERSE vs2 ++ [v] ++ vs1) = SOME (env',e) ∧
-   evaluate F env' s2 e bv
-      ⇒ evaluate_ctxt env s1 (Capp Opapp vs1 () es) v bv) ∧
+   (ck ⇒ s2.clock ≠ 0) ∧
+   evaluate ck env' (if ck then s2 with clock := s2.clock - 1 else s2) e bv
+      ⇒ evaluate_ctxt ck env s1 (Capp Opapp vs1 () es) v bv) ∧
 
-  (evaluate_list F env s1 es (s2, Rval vs2) ∧
+  (evaluate_list T env s1 es (s2, Rval vs2) ∧
+   do_opapp (REVERSE vs2 ++ [v] ++ vs1) = SOME (env',e) ∧
+   s2.clock = 0
+      ⇒ evaluate_ctxt T env s1 (Capp Opapp vs1 () es) v
+          (s2, Rerr (Rabort Rtimeout_error))) ∧
+
+  (evaluate_list ck env s1 es (s2, Rval vs2) ∧
    do_opapp (REVERSE vs2 ++ [v] ++ vs1) = NONE
-      ⇒ evaluate_ctxt env s1 (Capp Opapp vs1 () es) v
+      ⇒ evaluate_ctxt ck env s1 (Capp Opapp vs1 () es) v
           (s2, Rerr (Rabort Rtype_error))) ∧
 
   (op ≠ Opapp ∧
-   evaluate_list F env s1 es (s2, Rval vs2) ∧
+   evaluate_list ck env s1 es (s2, Rval vs2) ∧
    do_app (s2.refs,s2.ffi) op (REVERSE vs2 ++ [v] ++ vs1) =
     SOME ((new_refs, new_ffi) ,res)
-      ⇒ evaluate_ctxt env s1 (Capp op vs1 () es) v
+      ⇒ evaluate_ctxt ck env s1 (Capp op vs1 () es) v
           (s2 with <| ffi := new_ffi; refs := new_refs |>, res)) ∧
 
   (op ≠ Opapp ∧
-   evaluate_list F env s1 es (s2, Rval vs2) ∧
+   evaluate_list ck env s1 es (s2, Rval vs2) ∧
    do_app (s2.refs, s2.ffi) op (REVERSE vs2 ++ [v] ++ vs1) = NONE
-      ⇒ evaluate_ctxt env s1 (Capp op vs1 () es) v
+      ⇒ evaluate_ctxt ck env s1 (Capp op vs1 () es) v
           (s2, Rerr (Rabort Rtype_error))) ∧
 
-  (evaluate_list F env s es (s', Rerr err)
-      ⇒ evaluate_ctxt env s (Capp op vs () es) v (s', Rerr err)) ∧
+  (evaluate_list ck env s es (s', Rerr err)
+      ⇒ evaluate_ctxt ck env s (Capp op vs () es) v (s', Rerr err)) ∧
 
   (do_log lop v e2 = SOME (Exp e') ∧
-   evaluate F env s e' bv
-      ⇒ evaluate_ctxt env s (Clog lop () e2) v bv) ∧
+   evaluate ck env s e' bv
+      ⇒ evaluate_ctxt ck env s (Clog lop () e2) v bv) ∧
 
   (do_log lop v e2 = SOME (Val v')
-      ⇒ evaluate_ctxt env s (Clog lop () e2) v (s, Rval v')) ∧
+      ⇒ evaluate_ctxt ck env s (Clog lop () e2) v (s, Rval v')) ∧
 
 
   (do_log lop v e2 = NONE
-      ⇒ evaluate_ctxt env s (Clog lop () e2) v (s, Rerr (Rabort Rtype_error))) ∧
+      ⇒ evaluate_ctxt ck env s (Clog lop () e2) v (s, Rerr (Rabort Rtype_error))) ∧
 
   (do_if v e2 e3 = SOME e' ∧
-   evaluate F env s e' bv
-      ⇒ evaluate_ctxt env s (Cif () e2 e3) v bv) ∧
+   evaluate ck env s e' bv
+      ⇒ evaluate_ctxt ck env s (Cif () e2 e3) v bv) ∧
 
   (do_if v e2 e3 = NONE
-      ⇒ evaluate_ctxt env s (Cif () e2 e3) v (s, Rerr (Rabort Rtype_error))) ∧
+      ⇒ evaluate_ctxt ck env s (Cif () e2 e3) v (s, Rerr (Rabort Rtype_error))) ∧
 
-  (evaluate_match F env s v pes err_v bv
-      ⇒ evaluate_ctxt env s (Cmat () pes err_v) v bv) ∧
+  (evaluate_match ck env s v pes err_v bv
+      ⇒ evaluate_ctxt ck env s (Cmat () pes err_v) v bv) ∧
 
-  (evaluate_match F env s v pes err_v bv ∧
+  (evaluate_match ck env s v pes err_v bv ∧
    can_pmatch_all env.c s.refs (MAP FST pes) v
-      ⇒ evaluate_ctxt env s (Cmat_check () pes err_v) v bv) ∧
+      ⇒ evaluate_ctxt ck env s (Cmat_check () pes err_v) v bv) ∧
 
 
   (¬can_pmatch_all env.c s.refs (MAP FST pes) v
-      ⇒ evaluate_ctxt env s (Cmat_check () pes err_v) v
+      ⇒ evaluate_ctxt ck env s (Cmat_check () pes err_v) v
           (s, Rerr (Rabort Rtype_error))) ∧
 
-  (evaluate F (env with <| v := (nsOptBind n v env.v) |>) s e2 bv
-      ⇒ evaluate_ctxt env s (Clet n () e2) v bv) ∧
+  (evaluate ck (env with <| v := (nsOptBind n v env.v) |>) s e2 bv
+      ⇒ evaluate_ctxt ck env s (Clet n () e2) v bv) ∧
 
   (do_con_check env.c cn (LENGTH vs + LENGTH es + 1) ∧
    build_conv env.c cn (REVERSE vs' ++ [v] ++ vs) = SOME v' ∧
-   evaluate_list F env s1 es (s2, Rval vs')
-      ⇒ evaluate_ctxt env s1 (Ccon cn vs () es) v (s2, Rval v')) ∧
+   evaluate_list ck env s1 es (s2, Rval vs')
+      ⇒ evaluate_ctxt ck env s1 (Ccon cn vs () es) v (s2, Rval v')) ∧
 
   (¬do_con_check env.c cn (LENGTH vs + LENGTH es + 1)
-      ⇒ evaluate_ctxt env s (Ccon cn vs () es) v (s, Rerr (Rabort Rtype_error))) ∧
+      ⇒ evaluate_ctxt ck env s (Ccon cn vs () es) v (s, Rerr (Rabort Rtype_error))) ∧
 
   (do_con_check env.c cn (LENGTH vs + LENGTH es + 1) ∧
-   evaluate_list F env s es (s', Rerr err)
-      ⇒ evaluate_ctxt env s (Ccon cn vs () es) v (s', Rerr err)) ∧
+   evaluate_list ck env s es (s', Rerr err)
+      ⇒ evaluate_ctxt ck env s (Ccon cn vs () es) v (s', Rerr err)) ∧
 
-  evaluate_ctxt env s (Ctannot () t) v (s, Rval v) ∧
+  evaluate_ctxt ck env s (Ctannot () t) v (s, Rval v) ∧
 
-  evaluate_ctxt env s (Clannot () l) v (s, Rval v)
+  evaluate_ctxt ck env s (Clannot () l) v (s, Rval v)
 End
 
 Inductive evaluate_ctxts:
-  evaluate_ctxts s [] res (s, res) ∧
+  evaluate_ctxts ck s [] res (s, res) ∧
 
-  (evaluate_ctxt env s1 c v (s2, res) ∧
-   evaluate_ctxts s2 cs res bv
-      ⇒ evaluate_ctxts s1 ((c,env)::cs) (Rval v) bv) ∧
+  (evaluate_ctxt ck env s1 c v (s2, res) ∧
+   evaluate_ctxts ck s2 cs res bv
+      ⇒ evaluate_ctxts ck s1 ((c,env)::cs) (Rval v) bv) ∧
 
-  (evaluate_ctxts s cs (Rerr err) bv ∧
+  (evaluate_ctxts ck s cs (Rerr err) bv ∧
   ((∀pes. c ≠ Chandle () pes) ∨ (∀v. err ≠ Rraise v))
-      ⇒ evaluate_ctxts s ((c,env)::cs) (Rerr err) bv) ∧
+      ⇒ evaluate_ctxts ck s ((c,env)::cs) (Rerr err) bv) ∧
 
   (¬can_pmatch_all env.c s.refs (MAP FST pes) v ∧
-   evaluate_ctxts s cs (Rerr (Rabort Rtype_error)) res2
-      ⇒ evaluate_ctxts s ((Chandle () pes,env)::cs) (Rerr (Rraise v)) res2) ∧
+   evaluate_ctxts ck s cs (Rerr (Rabort Rtype_error)) res2
+      ⇒ evaluate_ctxts ck s ((Chandle () pes,env)::cs) (Rerr (Rraise v)) res2) ∧
 
-  (evaluate_match F env s v pes v (s', res1) ∧
+  (evaluate_match ck env s v pes v (s', res1) ∧
    can_pmatch_all env.c s.refs (MAP FST pes) v ∧
-   evaluate_ctxts s' cs res1 res2
-      ⇒ evaluate_ctxts s ((Chandle () pes,env)::cs) (Rerr (Rraise v)) res2)
+   evaluate_ctxts ck s' cs res1 res2
+      ⇒ evaluate_ctxts ck s ((Chandle () pes,env)::cs) (Rerr (Rraise v)) res2)
 End
 
 Inductive evaluate_state:
- (evaluate F env <| ffi := ffi; clock := 0; refs := refs; next_type_stamp := 0;
-                    next_exn_stamp := 0; eval_state := NONE |> e (st, res) ∧
-  evaluate_ctxts st c res bv
-      ⇒ evaluate_state (env, (refs, ffi), Exp e, c) bv) ∧
+ ((¬ck ⇒ clk = 0) ∧
+  evaluate ck env <| ffi := ffi; clock := clk; refs := refs; next_type_stamp := 0;
+                     next_exn_stamp := 0; eval_state := eval |> e (st, res) ∧
+  evaluate_ctxts ck st c res bv
+      ⇒ evaluate_state ck (env, (refs, ffi), Exp e, c) bv) ∧
 
- (evaluate_ctxts <| ffi := ffi; clock := 0; refs := refs; next_type_stamp := 0;
-                    next_exn_stamp := 0; eval_state := NONE |> c (Rval v) bv
-      ⇒ evaluate_state (env, (refs, ffi), Val v, c) bv)
+ ((¬ck ⇒ clk = 0) ∧
+  evaluate_ctxts ck <| ffi := ffi; clock := clk; refs := refs; next_type_stamp := 0;
+                       next_exn_stamp := 0; eval_state := eval |> c (Rval v) bv
+      ⇒ evaluate_state ck (env, (refs, ffi), Val v, c) bv)
 End
 
 val _ = export_theory()
